theories/logic/sem_sub_typing.v
@@ -19,7 +19,6 @@ From hazel.program_logic Require Import weakest_precondition
 From affine_tes.lang Require Import hazel.
 From affine_tes.lang Require Import subst_map.
 From affine_tes.logic Require Import sem_def.
-From affine_tes.logic Require Import tactics.
 From affine_tes.logic Require Import sem_types.
 From affine_tes.logic Require Import sem_env.
 
@@ -28,80 +27,67 @@ Section sub_typing.
 
   Context `{!heapGS Σ}.
 
-  Lemma sig_le_refl (ρ : sem_sig Σ) : ρ ≤R ρ.
+  Lemma sig_le_refl (ρ : sem_sig Σ) : ⊢ ρ ≤R ρ.
   Proof. iApply iEff_le_refl. Qed.
   
   Lemma sig_le_trans (ρ₁ ρ₂ ρ₃: sem_sig Σ) : 
-      ρ₁ ≤R ρ₂ →
-      ρ₂ ≤R ρ₃ →
+      ρ₁ ≤R ρ₂ -∗
+      ρ₂ ≤R ρ₃ -∗
       ρ₁ ≤R ρ₃. 
   Proof. 
-    intros Hρ₁₂ Hρ₂₃. 
-    iApply iEff_le_trans; [iApply Hρ₁₂|iApply Hρ₂₃]. 
+    iIntros "#Hρ₁₂ #Hρ₂₃". rewrite /sig_le /tc_opaque. 
+    iApply iEff_le_trans; [iApply "Hρ₁₂"|iApply "Hρ₂₃"]. 
   Qed.
   
   Lemma sigs_le_refl (ρs : sem_sigs Σ) :
-    ρs ≤Rs ρs.
-  Proof. destruct ρs. split; apply sig_le_refl. Qed.
+    ⊢ ρs ≤Rs ρs.
+  Proof. destruct ρs. iSplit; iApply sig_le_refl. Qed.
 
   Lemma sigs_le_trans (ρs₁ ρs₂ ρs₃ : sem_sigs Σ) :
-      ρs₁ ≤Rs ρs₂ →
-      ρs₂ ≤Rs ρs₃ →
+      ρs₁ ≤Rs ρs₂ -∗
+      ρs₂ ≤Rs ρs₃ -∗
       ρs₁ ≤Rs ρs₃. 
   Proof. 
-    intros Hρs₁₂ Hρs₂₃.
-    destruct ρs₁, ρs₂, ρs₃, Hρs₁₂, Hρs₂₃. split; by eapply sig_le_trans.
+    iIntros "#Hρs₁₂ #Hρs₂₃".
+    destruct ρs₁, ρs₂, ρs₃. 
+    iDestruct "Hρs₁₂" as "[H H']". 
+    iDestruct "Hρs₂₃" as "[? ?]". 
+    iSplit; simpl.  
+    { iApply sig_le_trans; [iApply "H"|iFrame "#"]. }
+    { iApply sig_le_trans; [iApply "H'"|iFrame "#"]. }
   Qed.
 
   Lemma sig_le_nil (ρ : sem_sig Σ) :
-    sem_sig_nil ≤R ρ.
-  Proof. apply iEff_le_bottom. Qed.
+    ⊢ sem_sig_nil ≤R ρ.
+  Proof. iApply iEff_le_bottom. Qed.
 
   Lemma sigs_le_nil (ρs : sem_sigs Σ) :
-    (⟨⟩ : sem_sigs Σ) ≤Rs ρs.
-  Proof. split; apply sig_le_nil. Qed.
+    ⊢ (⟨⟩ : sem_sigs Σ) ≤Rs ρs.
+  Proof. iSplit; iApply sig_le_nil. Qed.
   
   Lemma sigs_le_comp (ρ₁ ρ₂ ρ₁' ρ₂' : sem_sig Σ) :
-    ρ₁ ≤R ρ₁' →
-    ρ₂ ≤R ρ₂' →
+    ρ₁ ≤R ρ₁' -∗
+    ρ₂ ≤R ρ₂' -∗
     ⟨ ρ₁, ρ₂ ⟩ ≤Rs ⟨ ρ₁', ρ₂' ⟩.
-  Proof. intros ??. auto. Qed.
+  Proof. iIntros "??". iSplit; auto. Qed.
 
   Lemma sigs_le_os (ρ ρ' : sem_sig Σ) :
-    ρ ≤R ρ' →
+    ρ ≤R ρ' -∗
     (⟨ ρ , ⟩ : sem_sigs Σ) ≤Rs (⟨ ρ', ⟩ : sem_sigs Σ).
-  Proof. intros ?. split; first auto. apply sig_le_nil. Qed.
+  Proof. iIntros "?". iSplit; first auto. iApply sig_le_nil. Qed.
 
   Lemma sigs_le_ms (ρ ρ' : sem_sig Σ) :
-    ρ ≤R ρ' →
+    ρ ≤R ρ' -∗
     (⟨ , ρ ⟩ : sem_sigs Σ) ≤Rs (⟨ , ρ' ⟩ : sem_sigs Σ).
-  Proof. intros ?. split; last auto. apply sig_le_nil. Qed.
+  Proof. iIntros "?". iSplit; last auto. iApply sig_le_nil. Qed.
 
-  Lemma sig_le_eff_non_rec (ι₁ ι₂ κ₁ κ₂ : sem_ty Σ -n> sem_ty Σ) :
-    (∀ α, ι₁ α ≤T ι₂ α) →
-    (∀ α, κ₂ α ≤T κ₁ α) →
-    (μ∀TS: _ , α , ι₁ α ⇒ κ₁ α) ≤R (μ∀TS: _ , α , ι₂ α ⇒ κ₂ α).
-  Proof.
-    iIntros (Hι₁₂ Hκ₂₁ v Φ) "!#".
-    iPoseProof (sem_sig_eff_rec_eq OS (λ _ α, ι₂ α) (λ _ α, κ₂ α) v Φ) as "[_ Hrw]".
-    iIntros "Hμ₁". iApply "Hrw".
-    iPoseProof (sem_sig_eff_rec_eq OS (λ _ α, ι₁ α) (λ _ α, κ₁ α) v Φ) as "[Hrw' _]".
-    iDestruct ("Hrw'" with "Hμ₁") as "(%α & %w & <- & Hι₁ & HκΦ₁)".
-    iExists α, w; iSplitR; first done.
-    iSplitL "Hι₁".
-    { iNext. by iApply Hι₁₂. }
-    simpl. iIntros (b) "Hκ₂". iApply "HκΦ₁".
-    iNext. by iApply Hκ₂₁.
-  Qed.
-
-  (* TODO: For the recursive version we need ≤R and ≤T to live in iProp *)
   Lemma sig_le_eff_rec (ι₁ ι₂ κ₁ κ₂ : sem_sig Σ → sem_ty Σ → sem_ty Σ)
     `{NonExpansive2 ι₁, NonExpansive2 ι₂, NonExpansive2 κ₁, NonExpansive2 κ₂ } :
-    (∀ α ρ ρ', □ (iEff_le ρ ρ') -∗ □ (∀ v, (ι₁ ρ α) v -∗ (ι₂ ρ' α) v)) →
-    (∀ α ρ ρ', □ (iEff_le ρ ρ') -∗ □ (∀ v, (κ₂ ρ' α) v -∗ (κ₁ ρ α) v)) →
+    □ (∀ α ρ ρ', ρ ≤R ρ' -∗ (ι₁ ρ α) ≤T (ι₂ ρ' α)) -∗
+    □ (∀ α ρ ρ', ρ ≤R ρ' -∗ (κ₂ ρ' α) ≤T (κ₁ ρ α)) -∗
     (μ∀TS: θ , α , ι₁ θ α ⇒ κ₁ θ α) ≤R (μ∀TS: θ , α , ι₂ θ α ⇒ κ₂ θ α).
   Proof.
-    iIntros (Hι₁₂ Hκ₂₁). iLöb as "IH".
+    iIntros "#Hι₁₂ #Hκ₂₁". iLöb as "IH".
     iIntros (v Φ) "!#".
     iPoseProof (sem_sig_eff_rec_eq OS ι₂ κ₂ v Φ) as "[_ Hrw]".
     iIntros "Hμ₁". iApply "Hrw".
@@ -109,153 +95,157 @@ Section sub_typing.
     iDestruct ("Hrw'" with "Hμ₁") as "(%α & %w & <- & Hι₁ & HκΦ₁)".
     iExists α, w; iSplitR; first done.
     iSplitL "Hι₁".
-    { iNext. iApply (Hι₁₂ with "IH Hι₁"). }
+    { iNext. iApply ("Hι₁₂" with "IH Hι₁"). }
     simpl. iIntros (b) "Hκ₂". iApply "HκΦ₁".
-    iNext. iApply (Hκ₂₁ with "IH Hκ₂").
+    iNext. iApply ("Hκ₂₁" with "IH Hκ₂").
   Qed.
 
-  Lemma ty_le_refl (τ : sem_ty Σ) : τ ≤T τ.
-  Proof. done. Qed.
+  Lemma ty_le_refl (τ : sem_ty Σ) : ⊢ τ ≤T τ.
+  Proof. iIntros "!# % $". Qed.
   
   Lemma ty_le_trans (τ₁ τ₂ τ₃ : sem_ty Σ) :
-    τ₁ ≤T τ₂ →
-    τ₂ ≤T τ₃ →
+    τ₁ ≤T τ₂ -∗
+    τ₂ ≤T τ₃ -∗
     τ₁ ≤T τ₃.
   Proof. 
-    iIntros (Hτ₁₂ Hτ₂₃ v) "Hτ₁". 
-    iApply Hτ₂₃. by iApply Hτ₁₂.
+    iIntros "#Hτ₁₂ #Hτ₂₃ !# %v Hτ₁". 
+    iApply "Hτ₂₃". by iApply "Hτ₁₂".
   Qed.
   
-  Lemma ty_le_bot (τ : sem_ty Σ) :
-    ⊥ ≤T τ.
-  Proof. iIntros (?) "[]". Qed.
+  Lemma ty_le_void (τ : sem_ty Σ) :
+    ⊢ Void ≤T τ.
+  Proof. iIntros "% !# []". Qed.
 
   Lemma ty_le_cpy (τ : sem_ty Σ) :
-    copy_ty τ →
+    copy_ty τ -∗
     τ ≤T '! τ.
-  Proof. iIntros (? v). rewrite H. iIntros "#$". Qed.
-
+  Proof. 
+    iIntros "#Hcpy !# %v Hτ". 
+    iDestruct ("Hcpy" with "Hτ") as "#Hτ'".
+    iIntros "!# {$#Hτ'}". 
+  Qed.
+        
   Lemma ty_le_cpy_inv (τ : sem_ty Σ) :
-    ('! τ) ≤T τ.
-  Proof. iIntros (v) "#$". Qed.
+    ⊢ ('! τ) ≤T τ.
+  Proof. iIntros "!# %v #$". Qed.
 
   Lemma ty_le_u2aarr (τ κ : sem_ty Σ) (ρs : sem_sigs Σ) :
-    (τ -{ ρs }-> κ) ≤T (τ -{ ρs }-∘ κ).
+    ⊢ (τ -{ ρs }-> κ) ≤T (τ -{ ρs }-∘ κ).
   Proof.
-    iIntros (v) "#Hτκ". iIntros (w) "Hτ /=".
+    iIntros "!# %v #Hτκ". iIntros (w) "Hτ /=".
     iApply (ewp_pers_mono with "[Hτ Hτκ]"); [by iApply "Hτκ"|].
     iIntros "!# % $ //=".
   Qed.
 
   Lemma ty_le_aarr (τ₁ κ₁ τ₂ κ₂ : sem_ty Σ) (ρs ρs' : sem_sigs Σ) :
-    ρs ≤Rs ρs' →
-    τ₂ ≤T τ₁ →
-    κ₁ ≤T κ₂ →
+    ρs ≤Rs ρs' -∗
+    τ₂ ≤T τ₁ -∗
+    κ₁ ≤T κ₂ -∗
     (τ₁ -{ ρs }-∘ κ₁) ≤T (τ₂ -{ ρs' }-∘ κ₂).
   Proof.
-    iIntros ([Hρ₁ Hρ₂] Hτ₂₁ Hκ₁₂ v) "Hτκ₁ %w Hτ".
-    iApply ewp_os_prot_mono; [iApply Hρ₁|].
-    iApply ewp_ms_prot_mono; [iApply Hρ₂|].
+    iIntros "[#Hρ₁ #Hρ₂] #Hτ₂₁ #Hκ₁₂ !# %v Hτκ₁ %w Hτ".
+    iApply ewp_os_prot_mono; [iApply "Hρ₁"|].
+    iApply ewp_ms_prot_mono; [iApply "Hρ₂"|].
     iApply (ewp_pers_mono with "[Hτκ₁ Hτ]").
-    { iApply ("Hτκ₁" with "[Hτ]"); by rewrite Hτ₂₁. }
-    iIntros "!# % Hκ !>". by rewrite Hκ₁₂.
+    { iApply ("Hτκ₁" with "[Hτ]"); by iApply "Hτ₂₁". }
+    iIntros "!# % Hκ !>". by iApply "Hκ₁₂".
   Qed.
   
   Lemma ty_le_uarr (τ₁ κ₁ τ₂ κ₂ : sem_ty Σ) (ρs ρs' : sem_sigs Σ) :
-    ρs ≤Rs ρs' →
-    τ₂ ≤T τ₁ →
-    κ₁ ≤T κ₂ →
+    ρs ≤Rs ρs' -∗
+    τ₂ ≤T τ₁ -∗
+    κ₁ ≤T κ₂ -∗
     (τ₁ -{ ρs }-> κ₁) ≤T (τ₂ -{ ρs' }-> κ₂).
   Proof.
-    iIntros ([Hρ₁ Hρ₂] Hτ₂₁ Hκ₁₂ v) "#Hτκ₁ %w !# Hτ₂".
-    iApply ewp_os_prot_mono; [iApply Hρ₁|].
-    iApply ewp_ms_prot_mono; [iApply Hρ₂|].
+    iIntros "[#Hρ₁ #Hρ₂] #Hτ₂₁ #Hκ₁₂ !# %v #Hτκ₁ %w !# Hτ₂".
+    iApply ewp_os_prot_mono; [iApply "Hρ₁"|].
+    iApply ewp_ms_prot_mono; [iApply "Hρ₂"|].
     iApply (ewp_pers_mono with "[Hτκ₁ Hτ₂]").
-    { iApply ("Hτκ₁" with "[Hτ₂]"); by rewrite Hτ₂₁. }
-    iIntros "!# % Hκ !>". by rewrite Hκ₁₂.
+    { iApply ("Hτκ₁" with "[Hτ₂]"); by iApply "Hτ₂₁". }
+    iIntros "!# % Hκ !>". by iApply "Hκ₁₂".
   Qed.
   
   Lemma ty_le_ref (τ₁ τ₂ : sem_ty Σ) :
-    τ₁ ≤T τ₂ →
+    τ₁ ≤T τ₂ -∗
     (Ref τ₁) ≤T (Ref τ₂).
   Proof.
-    iIntros (Hτ₁₂ v) "(%l & -> & (%w & Hl & Hτw))".
+    iIntros "#Hτ₁₂ !# %v (%l & -> & (%w & Hl & Hτw))".
     iExists l. iSplit; first done.
-    iExists w. iFrame. by iApply Hτ₁₂.
+    iExists w. iFrame. by iApply "Hτ₁₂".
   Qed.
 
   Lemma ty_le_prod (τ₁ τ₂ κ₁ κ₂ : sem_ty Σ) :
-    τ₁ ≤T τ₂ →
-    κ₁ ≤T κ₂ →
+    τ₁ ≤T τ₂ -∗
+    κ₁ ≤T κ₂ -∗
     (τ₁ × κ₁) ≤T (τ₂ × κ₂).
   Proof.
-    iIntros (Hτ₁₂ Hκ₁₂ v) "(%w₁ & %w₂ & -> &Hw₁ & Hw₂)".
+    iIntros "#Hτ₁₂ #Hκ₁₂ !# %v (%w₁ & %w₂ & -> &Hw₁ & Hw₂)".
     iExists w₁, w₂. iSplit; first done. iSplitL "Hw₁".
-    { by iApply Hτ₁₂. }
-    by iApply Hκ₁₂.
+    { by iApply "Hτ₁₂". }
+    by iApply "Hκ₁₂".
   Qed.
   
   Lemma ty_le_sum (τ₁ τ₂ κ₁ κ₂ : sem_ty Σ) :
-    τ₁ ≤T τ₂ →
-    κ₁ ≤T κ₂ →
+    τ₁ ≤T τ₂ -∗
+    κ₁ ≤T κ₂ -∗
     (τ₁ + κ₁) ≤T (τ₂ + κ₂).
   Proof.
-    iIntros (Hτ₁₂ Hκ₁₂ v) "(%v' & [(-> & Hτ₁)|(-> & Hκ₁)])"; iExists v'. 
-    - iLeft. iSplit; first done. by iApply Hτ₁₂.
-    - iRight. iSplit; first done. by iApply Hκ₁₂. 
+    iIntros "#Hτ₁₂ #Hκ₁₂ !# %v (%v' & [(-> & Hτ₁)|(-> & Hκ₁)])"; iExists v'. 
+    - iLeft. iSplit; first done. by iApply "Hτ₁₂".
+    - iRight. iSplit; first done. by iApply "Hκ₁₂". 
   Qed.
 
   Lemma ty_le_option (τ₁ τ₂ : sem_ty Σ) :
-    τ₁ ≤T τ₂ →
+    τ₁ ≤T τ₂ -∗
     (Option τ₁) ≤T (Option τ₂).
-  Proof. intros ?. by apply ty_le_sum. Qed.
+  Proof. iIntros "#?". iApply ty_le_sum; last done. iIntros "!# % $". Qed.
 
   Lemma ty_le_forall ρs₁ ρs₂ (τ₁ τ₂ : sem_ty Σ → sem_sigs Σ → sem_ty Σ) :
-    ρs₁ ≤Rs ρs₂ →
-    (∀ α, τ₁ α ρs₁ ≤T τ₂ α ρs₂) →
+    ρs₁ ≤Rs ρs₂ -∗
+    (∀ α, τ₁ α ρs₁ ≤T τ₂ α ρs₂) -∗
     (∀T: α, ρs₁ , τ₁ α ρs₁)%T ≤T (∀T: α, ρs₂ , τ₂ α ρs₂).
   Proof.
-    iIntros ([Hρ₁ Hρ₂] Hτ₁₂ v) "#Hτ₁ %τ !#". unfold sem_ty_forall.
-    iApply ewp_os_prot_mono; [iApply Hρ₁|].
-    iApply ewp_ms_prot_mono; [iApply Hρ₂|].
+    iIntros "[#Hρ₁ #Hρ₂] #Hτ₁₂ !# %v #Hτ₁ %τ !#". unfold sem_ty_forall.
+    iApply ewp_os_prot_mono; [iApply "Hρ₁"|].
+    iApply ewp_ms_prot_mono; [iApply "Hρ₂"|].
     iApply (ewp_pers_mono with "[Hτ₁]"); [iApply "Hτ₁"|].
-    iIntros "!# % Hτ !>". by iApply Hτ₁₂.
+    iIntros "!# % Hτ !>". by iApply "Hτ₁₂".
   Qed.
 
   Lemma ty_le_sig_forall (τ₁ τ₂ : sem_sigs Σ → sem_ty Σ) :
-    (∀ θ, τ₁ θ ≤T τ₂ θ) →
-    (∀S: θ, τ₁ θ) ≤T (∀S: θ, τ₂ θ).
+    (∀ θ, τ₁ θ ≤T τ₂ θ) -∗
+    (∀R: θ, τ₁ θ) ≤T (∀R: θ, τ₂ θ).
   Proof.
-    iIntros (Hτ₁₂ v) "Hτ₁ %ρ".
+    iIntros "#Hτ₁₂ !# %v #Hτ₁ %ρ !#".
     iApply (ewp_pers_mono with "[Hτ₁]"); [iApply "Hτ₁"|].
-    iIntros "!# % Hτ₁ !>".
-    iApply (Hτ₁₂ ρ with "Hτ₁").
+    iIntros "!# % Hτ₁ρ !>".
+    iApply ("Hτ₁₂" $! ρ with "Hτ₁ρ").
   Qed.
 
   Lemma ty_le_exists (τ₁ τ₂ : sem_ty Σ → sem_ty Σ) :
-    (∀ α, τ₁ α ≤T τ₂ α) →
+    (∀ α, τ₁ α ≤T τ₂ α) -∗
     (∃: α, τ₁ α) ≤T (∃: α, τ₂ α).
   Proof.
-    iIntros (Hτ₁₂ v) "(%α & Hα) //=".
-    iExists α. by iApply Hτ₁₂.
+    iIntros "#Hτ₁₂ !# %v (%α & Hα) //=".
+    iExists α. by iApply "Hτ₁₂".
   Qed.
 
-  (* TODO: For recursive type sub-typing we need ≤T to live in iProp *)
   Lemma ty_le_rec (τ₁ τ₂ : sem_ty Σ -> sem_ty Σ) `{NonExpansive τ₁, NonExpansive τ₂} :
-    (∀ α α', □ (∀ v, α v -∗ α' v) -∗ □ ∀ v, τ₁ α v -∗ τ₂ α' v) →
+    □ (∀ α α', (α ≤T α') -∗ τ₁ α ≤T τ₂ α') -∗
     (μT: α, τ₁ α) ≤T (μT: α, τ₂ α).
   Proof.
-    iIntros (Hτ₁₂). iLöb as "IH". iIntros "%v Hτ₁".
+    iIntros "#Hτ₁₂ !#". iLöb as "IH". iIntros "%v Hτ₁".
     iApply sem_ty_rec_unfold.
     rewrite sem_ty_rec_unfold. iNext.
-    iApply (Hτ₁₂ with "IH Hτ₁").
+    iApply ("Hτ₁₂" with "[] Hτ₁").
+    rewrite /ty_le /tc_opaque. iApply "IH".
   Qed.
 
   Lemma ty_le_list (τ₁ τ₂ : sem_ty Σ) :
-    τ₁ ≤T τ₂ →
+    τ₁ ≤T τ₂ -∗
     List τ₁ ≤T List τ₂.
   Proof.
-    iIntros (Hτ₁₂ v) "HLτ₁". unfold sem_ty_list.
+    iIntros "#Hτ₁₂ !# %v HLτ₁". unfold sem_ty_list.
     iLöb as "IH" forall (v).
     iApply sem_ty_rec_unfold.
     rewrite sem_ty_rec_unfold. iNext.
@@ -263,47 +253,47 @@ Section sub_typing.
     { iExists v'; iLeft. by iFrame. }
     iExists (w₁, w₂)%V. iRight. iSplit; first done.
     iExists w₁, w₂; iSplit; first done.
-    iSplitL "Hτ₁"; [by iApply Hτ₁₂|by iApply "IH"].
+    iSplitL "Hτ₁"; [by iApply "Hτ₁₂"|by iApply "IH"].
   Qed.
   
-  Lemma env_le_refl Γ : Γ ≤E Γ.
-  Proof. done. Qed.
+  Lemma env_le_refl Γ : ⊢ Γ ≤E Γ.
+  Proof. iIntros "!# % $". Qed.
   
   Lemma env_le_trans Γ₁ Γ₂ Γ₃ : 
-    Γ₁ ≤E Γ₂ →
-    Γ₂ ≤E Γ₃ →
+    Γ₁ ≤E Γ₂ -∗
+    Γ₂ ≤E Γ₃ -∗
     Γ₁ ≤E Γ₃.
   Proof.
-    iIntros (HΓ₁₂ HΓ₂₃ vs) "HΓ₁ //=".  
-    iApply HΓ₂₃. by iApply HΓ₁₂.
+    iIntros "#HΓ₁₂ #HΓ₂₃ !# %vs HΓ₁ //=".  
+    iApply "HΓ₂₃". by iApply "HΓ₁₂".
   Qed.
   
   Lemma env_le_cons Γ₁ Γ₂ τ₁ τ₂ x :
-    Γ₁ ≤E Γ₂ →
-    τ₁ ≤T τ₂ →
+    Γ₁ ≤E Γ₂ -∗
+    τ₁ ≤T τ₂ -∗
     (x, τ₁) :: Γ₁ ≤E (x, τ₂) :: Γ₂.
   Proof.
-    iIntros (HΓ₁₂ Hτ₁₂ vs) "[%v (Hlookup & Hv & HΓ₁)]".
-    iExists v. iFrame. iSplitR "HΓ₁"; last (by iApply HΓ₁₂).
-    by iApply Hτ₁₂.
+    iIntros "#HΓ₁₂ #Hτ₁₂ !# %vs [%v (Hlookup & Hv & HΓ₁)]".
+    iExists v. iFrame. iSplitR "HΓ₁"; last (by iApply "HΓ₁₂").
+    by iApply "Hτ₁₂".
   Qed.
   
   Lemma env_le_copy_contraction Γ x τ :
-    copy_ty τ →
+    copy_ty τ -∗
     (x, τ) :: Γ ≤E (x, τ) :: (x, τ) :: Γ.
   Proof.
-    move =>Hcpyτ vs.
+    iIntros "#Hcpy !# %vs".
     iIntros "//= [%w (%Hrw & Hτ & HΓ)]". 
-    rewrite Hcpyτ. iDestruct "Hτ" as "#Hτ".
+    iDestruct ("Hcpy" with "Hτ") as "#Hτ'".
     by do 2 (iExists w; iFrame "%#").
   Qed.
   
   Lemma env_le_bring_forth Γ n x τ :
     nth_error Γ n = Some (x, τ) →
-    Γ ≤E (x, τ) :: (list_delete n Γ) .
+    ⊢ Γ ≤E (x, τ) :: (list_delete n Γ) .
   Proof.
     iInduction n as [|] "IH" forall (Γ); iIntros (Hnth vs);
-    iIntros "HΓ"; simpl in Hnth; destruct Γ; first done; simplify_eq; first done.
+    iIntros "!# HΓ"; simpl in Hnth; destruct Γ; first done; simplify_eq; first done.
     destruct p; simpl. rewrite !env_sem_typed_cons.
     iDestruct "HΓ" as "[$ HΓ]". rewrite -env_sem_typed_cons.
     by iApply "IH". 
@@ -311,52 +301,52 @@ Section sub_typing.
 
   Lemma env_le_bring_forth_rev Γ n x τ :
     nth_error Γ n = Some (x, τ) →
-    (x, τ) :: (list_delete n Γ) ≤E Γ.
+    ⊢ (x, τ) :: (list_delete n Γ) ≤E Γ.
   Proof.
     iInduction n as [|] "IH" forall (Γ); iIntros (Hnth vs);
     simpl in Hnth; 
     destruct Γ as [|[y κ] Γ']; first done; 
-    simplify_eq; simpl; first (iIntros "$").
-    iIntros "[%v (? & ? & [%w (? & ? & ?)])]". 
+    simplify_eq; simpl; first (iIntros "!# $").
+    iIntros "!# [%v (? & ? & [%w (? & ? & ?)])]". 
     iExists w. iFrame. iApply "IH"; first done.
     iExists v. iFrame.
   Qed.
 
   Lemma env_le_swap_second Γ x y τ₁ τ₂ : 
-    (y, τ₂) :: (x, τ₁) :: Γ ≤E (x, τ₁) :: (y, τ₂) :: Γ.
+    ⊢ (y, τ₂) :: (x, τ₁) :: Γ ≤E (x, τ₁) :: (y, τ₂) :: Γ.
   Proof.
     pose proof (env_le_bring_forth_rev ((x, τ₁) :: (y, τ₂) :: Γ) 1 y τ₂).
     by apply H.
   Qed.
 
   Lemma env_le_swap_third Γ x y z τ₁ τ₂ τ₃: 
-    (z, τ₃) :: (x, τ₁) :: (y, τ₂) :: Γ ≤E (x, τ₁) :: (y, τ₂) :: (z, τ₃) :: Γ.
+    ⊢ (z, τ₃) :: (x, τ₁) :: (y, τ₂) :: Γ ≤E (x, τ₁) :: (y, τ₂) :: (z, τ₃) :: Γ.
   Proof.
     pose proof (env_le_bring_forth_rev ((x, τ₁) :: (y, τ₂) :: (z, τ₃) :: Γ) 2 z τ₃).
     by apply H.
   Qed.
 
   Lemma env_le_swap_fourth Γ x y z z' τ₁ τ₂ τ₃ τ₄: 
-    (z', τ₄) :: (x, τ₁) :: (y, τ₂) :: (z, τ₃) :: Γ ≤E (x, τ₁) :: (y, τ₂) :: (z, τ₃) :: (z', τ₄) :: Γ.
+    ⊢ (z', τ₄) :: (x, τ₁) :: (y, τ₂) :: (z, τ₃) :: Γ ≤E (x, τ₁) :: (y, τ₂) :: (z, τ₃) :: (z', τ₄) :: Γ.
   Proof.
     pose proof (env_le_bring_forth_rev ((x, τ₁) :: (y, τ₂) :: (z, τ₃) :: (z', τ₄) :: Γ) 3 z' τ₄).
     by apply H.
   Qed.
 
   Lemma env_le_swap_env_singl Γ x τ : 
-    (x, τ) :: Γ ≤E Γ ++ [(x, τ)].
+    ⊢ (x, τ) :: Γ ≤E Γ ++ [(x, τ)].
   Proof.
     induction Γ as [|[y κ] Γ'].
-    { solve_env. }
+    { simpl. iIntros "!# % $". }
     rewrite -app_comm_cons.
-    eapply env_le_trans; [apply env_le_swap_second|].
-    apply env_le_cons; last done.
-    apply IHΓ'.
+    iApply env_le_trans; [iApply env_le_swap_second|].
+    iApply env_le_cons; last (iIntros "!# % $").
+    iApply IHΓ'.
   Qed.
 
   Lemma env_le_weaken Γ x τ :
-    (x, τ) :: Γ ≤E Γ.
-  Proof. iIntros (?) "[% (? & ? & $)]". Qed.
+    ⊢ (x, τ) :: Γ ≤E Γ.
+  Proof. iIntros "!# % [% (? & ? & $)]". Qed.
 
 End sub_typing.
 
@@ -368,85 +358,97 @@ Section copyable_types.
   
   Open Scope sem_ty_scope.
 
-  Lemma copy_ty_unit : copy_ty ().
-  Proof. solve_copy. Qed.
+  Lemma copy_ty_void : ⊢ copy_ty Void.
+  Proof. iIntros "!# %v $!". Qed.
+
+  Lemma copy_ty_unit : ⊢ copy_ty ().
+  Proof. iIntros "!# %v $!". Qed.
   
-  Lemma copy_ty_bool : copy_ty 𝔹.
-  Proof. solve_copy. Qed.
+  Lemma copy_ty_bool : ⊢ copy_ty 𝔹.
+  Proof. iIntros "!# %v #$". Qed.
   
-  Lemma copy_ty_nat : copy_ty ℤ.
-  Proof. solve_copy. Qed.
+  Lemma copy_ty_nat : ⊢ copy_ty ℤ.
+  Proof. iIntros "!# %v #$". Qed.
   
-  Lemma copy_ty_moved : copy_ty Moved.
-  Proof. solve_copy. Qed.
+  Lemma copy_ty_moved : ⊢ copy_ty Moved.
+  Proof. iIntros "!# %v #$". Qed.
 
-  Lemma copy_ty_cpy τ : copy_ty ('! τ).
-  Proof. solve_copy. Qed.
+  Lemma copy_ty_cpy τ : ⊢ copy_ty ('! τ).
+  Proof. iIntros "!# %v #$". Qed.
 
-  Lemma copy_ty_uarr τ ρ κ : copy_ty (τ -{ ρ }-> κ).
-  Proof. solve_copy. Qed.
+  Lemma copy_ty_uarr τ ρ κ : ⊢ copy_ty (τ -{ ρ }-> κ).
+  Proof. iIntros "!# %v #$". Qed.
   
-  Lemma copy_ty_prod τ κ : copy_ty τ → copy_ty κ → copy_ty (τ × κ).
-  Proof. by solve_copy. Qed.
-  
-  Lemma copy_ty_sum τ κ : copy_ty τ → copy_ty κ → copy_ty (τ + κ).
-  Proof. by solve_copy. Qed.
+  Lemma copy_ty_prod τ κ : copy_ty τ -∗ copy_ty κ -∗ copy_ty (τ × κ).
+  Proof. 
+    iIntros "#Hcpyτ #Hcpyκ !# %v (% & % & -> & Hτ & Hκ)". 
+    iDestruct ("Hcpyτ" with "Hτ") as "#Hτ'".
+    iDestruct ("Hcpyκ" with "Hκ") as "#Hκ'". 
+    iIntros "!#". iExists v₁, v₂. by iFrame "#".
+  Qed.
 
-  Lemma copy_ty_forall C ρs : copy_ty (∀T: α, ρs , C α).
-  Proof. by solve_copy. Qed.
+  Lemma copy_ty_sum τ κ : copy_ty τ -∗ copy_ty κ -∗ copy_ty (τ + κ).
+  Proof.
+    iIntros "#Hcpyτ #Hcpyκ !# %v (% & [(-> & Hτ)|(-> & Hκ)])". 
+    - iDestruct ("Hcpyτ" with "Hτ") as "#Hτ'". iIntros "!#". 
+      iExists v'. iLeft. by iFrame "#".
+    - iDestruct ("Hcpyκ" with "Hκ") as "#Hκ'". iIntros "!#". 
+      iExists v'. iRight. by iFrame "#".
+  Qed.
 
-  Lemma copy_ty_ref τ : copy_ty (Refᶜ τ).
-  Proof. by solve_copy. Qed.
+  Lemma copy_ty_forallT C ρs : ⊢ copy_ty (∀T: α, ρs , C α).
+  Proof. iIntros "!# % #$". Qed.
 
-  Lemma copy_ty_option τ : copy_ty τ → copy_ty (Option τ).
-  Proof. by solve_copy. Qed.
+  Lemma copy_ty_forallR C : ⊢ copy_ty (∀R: θ, C θ).
+  Proof. iIntros "!# % #$". Qed.
 
-  Lemma copy_ty_exists τ : (∀ α, copy_ty (τ α)) → copy_ty (∃: α, τ α).
-  Proof. solve_copy. apply H. Qed.
+  Lemma copy_ty_ref τ : ⊢ copy_ty (Refᶜ τ).
+  Proof. iIntros "!# % #$". Qed.
+
+  Lemma copy_ty_exists τ : (∀ α, copy_ty (τ α)) -∗ copy_ty (∃: α, τ α).
+  Proof. 
+    iIntros "#H !# % [%α Hτ']". 
+    iDestruct ("H" with "Hτ'") as "#Hτ".
+    iIntros "!#". by iExists α.
+  Qed.
 
   Lemma copy_ty_rec τ `{NonExpansive τ}: 
-    (∀ α, copy_ty (τ α)) → copy_ty (μT: α, τ α).
+    □ (∀ α, (copy_ty α) -∗ copy_ty (τ α)) -∗ 
+    copy_ty (μT: α, τ α).
   Proof. 
-    iIntros (H v). rewrite sem_ty_rec_unfold.
-    solve_copy. apply H. 
+    iIntros "#H !# %". iLöb as "IH" forall (v). 
+    rewrite {1 2} sem_ty_rec_unfold.
+    iIntros "Hτ". iApply bi.later_intuitionistically.
+    iNext. iApply ("H" with "[] Hτ"). 
+    rewrite /copy_ty /tc_opaque. iApply "IH".
   Qed.
 
-  Lemma copy_ty_list τ : copy_ty τ → copy_ty (List τ).
+  Lemma copy_ty_option τ : copy_ty τ -∗ copy_ty (Option τ).
+  Proof. 
+    iIntros "#H". 
+    iApply copy_ty_sum; [iApply copy_ty_unit|done]. 
+  Qed.
+
+  Lemma copy_ty_list τ : copy_ty τ -∗ copy_ty (List τ).
   Proof.
-    iIntros (Hcpyτ). unfold sem_ty_list. unfold copy_ty.
-    iIntros (v). unfold Persistent. iIntros "Hμ".
-    iLöb as "IH" forall (v).
-    rewrite sem_ty_rec_unfold. rewrite -bi.later_persistently_1.
-    iNext. unfold ListF.
-    rewrite bi.persistently_exist. 
-    iDestruct "Hμ" as "(%w & [(-> & #Hunit)|(-> & (%w₁ & %w₂ & -> & Hτ & Hμ))])".
-    { iExists w; rewrite bi.persistently_or;
-      iLeft. iIntros "!# {$Hunit} //=". }
-    iExists (w₁, w₂)%V. rewrite bi.persistently_or.
-    iRight. unfold copy_ty in Hcpyτ. rewrite Hcpyτ.
-    iDestruct "Hτ" as "#Hτ".
-    iDestruct ("IH" with "Hμ") as "#Hμ₂".
-    iIntros "!#". iSplit; first done.
-    iExists w₁, w₂; iSplit; first done. by iSplit.
+    iIntros "#Hτ". iApply copy_ty_rec.
+    iIntros "!# % #Hα". 
+    iApply copy_ty_sum; [iApply copy_ty_unit|].
+    by iApply copy_ty_prod.
   Qed.
 
-  Lemma copy_env_nil : copy_env [].
-  Proof. solve_copy. Qed.
+  Lemma copy_env_nil : ⊢ copy_env [].
+  Proof. iIntros "!# % #$". Qed.
   
   Lemma copy_env_cons Γ x τ : 
-    copy_env Γ →
-    copy_ty τ →
+    copy_env Γ -∗
+    copy_ty τ -∗
     copy_env ((x, τ) :: Γ).
   Proof. 
-    intros ???. rewrite env_sem_typed_cons.
-    by solve_copy. Qed.
-
-  Lemma copy_pers τ :
-    ⌜ copy_ty τ ⌝ -∗ □ (∀ v, τ v -∗ □ (τ v)).
-  Proof.
-    iIntros "%Hcpy !# %v Hτ".
-    unfold copy_ty, Persistent in Hcpy. 
-    by iDestruct (Hcpy v with "Hτ") as "#Hτv".
+    iIntros "#HΓcpy #Hτcpy !# % (% & %Hrw & Hτ & HΓ)".
+    iDestruct ("Hτcpy" with "Hτ") as "#Hτ'".
+    iDestruct ("HΓcpy" with "HΓ") as "#HΓ'".
+    iIntros "!#". iExists v. by iFrame "#".
   Qed.
 
 End copyable_types.
